take_write_lock method

examples/scache/Cache.i.dfy
@@ -1,7 +1,87 @@
+include "AtomicRefcount.i.dfy"
+include "AtomicStatus.i.dfy"
+
 module CacheImpl {
+  import opened Constants
+  import opened AtomicStatusImpl
+  import opened AtomicRefcountImpl
+  import opened Ptrs
+  import opened LinearMaybe
+
   datatype Cache = Cache(
     data: seq<Ptr>,
     status: seq<AtomicStatus>,
-    read_locks: seq<seq<AtomicRefcount>
+    read_refcounts: seq<seq<AtomicRefcount>>
   )
+
+  predicate Inv(c: Cache)
+  {
+    && |c.data| == CacheSize()
+    && |c.status| == CacheSize()
+    && (forall i | 0 <= i < CacheSize() ::
+       atomic_status_inv(c.status[i], c.data[i]))
+    && |c.read_refcounts| == NThreads()
+    && (forall j | 0 <= j < NThreads() ::
+        |c.read_refcounts[j]| == CacheSize())
+    && (forall j, i | 0 <= j < NThreads() && 0 <= i < CacheSize() ::
+        atomic_refcount_inv(c.read_refcounts[j][i], c.data[i], j))
+  }
+
+  method take_write_lock(c: Cache, cache_idx: int)
+  returns (linear w: ReadWriteLockResources.Q)
+  requires Inv(c)
+  requires 0 <= cache_idx < CacheSize()
+  decreases *
+  {
+    linear var w_maybe := empty();
+    var success := false;
+
+    while !success 
+    invariant success ==> w_maybe == give(
+        ReadWriteLockResources.WritePendingAwaitBack(c.data[cache_idx]))
+    invariant !success ==> !has(w_maybe)
+    decreases *
+    {
+      var _ := discard(w_maybe);
+      success, w_maybe := try_set_write_lock(
+          c.status[cache_idx], c.data[cache_idx]);
+    }
+
+    w := unwrap(w_maybe);
+
+    success := false;
+
+    while !success 
+    invariant !success ==> w ==
+        ReadWriteLockResources.WritePendingAwaitBack(c.data[cache_idx])
+    invariant success ==> w ==
+        ReadWriteLockResources.WritePending(c.data[cache_idx], 0)
+    decreases *
+    {
+      success, w := try_check_writeback_isnt_set(
+          c.status[cache_idx], c.data[cache_idx], w);
+    }
+
+    var j := 0;
+    while j < NThreads()
+    invariant 0 <= j <= NThreads()
+    invariant w == 
+        ReadWriteLockResources.WritePending(c.data[cache_idx], j)
+    {
+      success := false;
+
+      while !success 
+      invariant !success ==> w ==
+          ReadWriteLockResources.WritePending(c.data[cache_idx], j)
+      invariant success ==> w ==
+          ReadWriteLockResources.WritePending(c.data[cache_idx], j+1)
+      decreases *
+      {
+        success, w := is_refcount_zero(c.read_refcounts[j][cache_idx],
+            c.data[cache_idx], j, w);
+      }
+
+      j := j + 1;
+    }
+  }
 }
